lakefile.lean
@@ -15,5 +15,5 @@ lean_lib Freigen where
 lean_exe freigen where
   root := `Main
 
-lean_exe sha2562kb_bench where
-  root := `BenchSha2562KB
+lean_exe sha256_fast_witgen_bench where
+  root := `BenchSha256FastWitgen
